\section{Apendiks B: Tablica integrala}

\definecolor{c_constant}{HTML}{d98530}

\begin{center}
    
\vspace*{\stretch{1}}

\begin{align*}
    \int {\color{accent}a}\,dx =&\, {\color{accent}a\cdot x} + {\color{c_constant}C}\\
    \int {\color{accent}x^a} \,dx =&\, {\color{accent}\frac{x^{a+1}}{a+1}} + {\color{c_constant}C}\,,\quad a \neq 1\\
    \int {\color{accent}\frac{1}{x}}\,dx =&\, {\color{accent}\ln |x|} + {\color{c_constant}C}\\
    \int {\color{accent} e^x} \,dx =&\, {\color{accent} e^x} + {\color{c_constant}C}\\
    \int {\color{accent} a^x} \,dx =&\, {\color{accent} \frac{a^x}{\ln a}} + {\color{c_constant}C}
\end{align*}

\vspace*{\stretch{0.8}}

\begin{multicols}{2}
    \vspace*{\stretch{1}}
    \begin{align*}
        \int {\color{accent} \cos x}\,dx =&\,{\color{accent} \sin x} + {\color{c_constant}C}\\
        \int {\color{accent} \sin x}\,dx =&\,-{\color{accent} \cos x} + {\color{c_constant}C}\\
        \int {\color{accent} \frac{1}{\cos^2x}}\,dx =&\,{\color{accent} \tan x} + {\color{c_constant}C}\\
        \int {\color{accent} \frac{1}{\sin^2x}}\,dx =&\,-{\color{accent} \cot x}
    \end{align*}
    \vspace*{\stretch{1}}

    \columnbreak

    \vspace*{\stretch{1}}
    \begin{align*}
        \int {\color{accent} \frac{1}{\sqrt{1 - x^2}}}\,dx = &\,{\color{accent} \arcsin x} + {\color{c_constant}C} \,,&&a > 0\\
        \int {\color{accent} \frac{1}{a^x + x^2}}\,dx = &\,{\color{accent} \dfrac{\arctan \dfrac{x}{a}}{a}} + {\color{c_constant}C}\,,&&a > 0
    \end{align*}
    \vspace*{\stretch{1}}
\end{multicols}

\begin{multicols}{2}
    \vspace*{\stretch{1}}
    \begin{align*}
        \int \text{ch}\, x\,dx =&\,\text{sh}\, x + {\color{c_constant}C}\\
        \int \text{sh}\, x\,dx =&\,\text{ch}\, x + {\color{c_constant}C}\\
        \int \frac{1}{\text{ch}^2 x}\,dx =&\,\text{th}\, x + {\color{c_constant}C}\\
        \int \frac{1}{\text{sh}^2 x}\,dx =&\,-\text{cth}\, x + {\color{c_constant}C}
    \end{align*}
    \vspace*{\stretch{1}}

    \columnbreak

    \vspace*{\stretch{1}}
    \begin{align*}
        \frac{1}{\sqrt{1 - x^2}}=&\,\text{Arsh}\, x  + {\color{c_constant}C} = \ln (x+\sqrt{1+x^2}) + {\color{c_constant}C}\\
        \frac{1}{\sqrt{x^2 - 1}}=&\,\text{Arch}\, x  + {\color{c_constant}C} = \ln |x+\sqrt{x^2-1})| + {\color{c_constant}C}
    \end{align*}
    \vspace*{\stretch{1}}
\end{multicols}

\vspace*{\stretch{1}}

\end{center}