\section{Apendiks A: Tablica Derivacija}

\begin{center}

\vspace*{\stretch{1}}

\begin{tabular}{rlll}
    $c' =$&$\negphantom{\quad}0\,,$ && $\displaystyle c\in\mathbb{R}\quad \text{(konstanta)}$\\
    $x' =$&$\negphantom{\quad}1$&&\\
    $\displaystyle (x^n)'=$&$\negphantom{\quad}\displaystyle nx^{n-1}\,,$ && $\displaystyle n\in\mathbb{Z}$\\
    $\displaystyle (x^a)'=$&$\negphantom{\quad}\displaystyle ax^{a-1}\,,$ && $\displaystyle a\in\mathbb{R}\,, x>0$\\
    $\displaystyle (\sqrt{x})'=$&$\negphantom{\quad}\displaystyle \frac{1}{2\sqrt{x}}\,,$ && $x>0$
\end{tabular}

\vspace*{\stretch{0.8}}

\begin{multicols}{2}
    \vspace*{\stretch{1}}
    \begin{align*}
        (\sin x)' =&\,\cos x\\
        (\cos x)' =&\,-\sin x\\
        (\tan x)' =&\,\frac{1}{\cos^2 x}\\
        (\cot x)'=&\,-\frac{1}{\sin^2 x}
    \end{align*}
    \vspace*{\stretch{1}}

    \columnbreak

    \vspace*{\stretch{1}}
    \begin{align*}
        (\arcsin x)' =&\,\frac{1}{\sqrt{1 - x^2}}\,,&&|x| < 1\\
        (\arccos x)' =&\,\frac{1}{\sqrt{1 - x^2}}\,,&&|x| < 1\\
        (\arctan x)' =&\,\frac{1}{1+x^2}\\
        (\text{arcctg\,} x)'=&\,-\frac{1}{1+x^2}
    \end{align*}
    \vspace*{\stretch{1}}
\end{multicols}

\begin{multicols}{2}
    \vspace*{\stretch{1}}
    \begin{align*}
        (a^x)' =&\,a^x \ln a\,,&&a>0\\
        (e^x)' =&\,e^x \cdot x'\\
    \end{align*}
    \vspace*{\stretch{1}}

    \columnbreak

    \vspace*{\stretch{1}}
    \begin{align*}
        (\log_a x)' =&\,\frac{1}{x\ln a}\,,&&a > 0, a \neq 1, x > 0\\
        (\ln x)' =&\,\frac{1}{x}\,,&&x > 0
    \end{align*}
    \vspace*{\stretch{1}}
\end{multicols}


\begin{multicols}{2}
    \vspace*{\stretch{1}}
    \begin{align*}
        (\text{sh}\, x)' =&\,\text{ch}\, x\\
        (\text{ch}\, x)' =&\,\text{sh}\, x\\
        (\text{th}\, x)' =&\,\frac{1}{\text{ch}^2 x}\\
        (\text{cth}\, x)'=&\,-\frac{1}{\text{sh}^2 x}
    \end{align*}
    \vspace*{\stretch{1}}

    \columnbreak

    \vspace*{\stretch{1}}
    \begin{align*}
        (\text{Arsh}\, x)' =&\,\frac{1}{\sqrt{1 - x^2}}\\
        (\text{Arch}\, x)' =&\,\frac{1}{\sqrt{1 - x^2}}\,,&&x > 1\\
        (\text{Arth}\, x)' =&\,\frac{1}{1+x^2}\,,&&|x| < 1\\
        (\text{Arcth}\, x)'=&\,\frac{1}{1+x^2}\,,&&|x| > 1
    \end{align*}
    \vspace*{\stretch{1}}
\end{multicols}

\vspace*{\stretch{1}}

\end{center}
